Foundation/Propositional/Logic/PostComplete.lean
@@ -1,0 +1,43 @@
+import Foundation.Propositional.Hilbert.WellKnown
+import Foundation.Propositional.Kripke.Logic.Cl
+import Foundation.Propositional.Logic.Extension
+import Foundation.Propositional.ClassicalSemantics.Hilbert
+import Foundation.Propositional.ClassicalSemantics.ZeroSubst
+
+-- #check Set.ssubset_of_subset
+
+lemma Set.ssubset_of_subset_ne {α : Type*} {s t : Set α} (h : s ⊆ t) (hne : s ≠ t) : s ⊂ t := by
+  constructor;
+  . assumption;
+  . revert hne;
+    contrapose!;
+    intro _;
+    apply Set.eq_of_subset_of_subset <;> assumption;
+
+namespace LO.Propositional
+
+namespace Logic
+
+abbrev Ext (L : Logic) := { L' : Logic // L'.Superintuitionistic ∧ L ⊆ L' }
+
+open Formula (atom)
+open Formula.ClassicalSemantics
+open Propositional.Hilbert.Cl
+open Superintuitionistic
+open ClassicalSemantics
+
+theorem Cl.post_complete : ∀ L : Ext (Logic.Cl), L.1.Consistent → L.1 = Logic.Cl := by
+  by_contra! hC;
+  obtain ⟨⟨L, L_si, L_subset⟩, L_consis, L_ne⟩ := hC;
+  apply Logic.no_bot (L := L);
+  replace ⟨hL, ⟨φ, hφ₁, hφ₂⟩⟩ := Set.ssubset_iff_exists.mp $ Set.ssubset_of_subset_ne L_subset (by tauto);
+  have ⟨v, hv⟩ := exists_valuation_of_not_provable hφ₂;
+  have h₁ : ∼(φ⟦(vfSubst v).1⟧) ∈ L := hL $ by
+    apply Hilbert.Cl.completeness;
+    sorry;
+  have h₂ : φ⟦(vfSubst v).1⟧ ∈ L := subst_closed hφ₁ _;
+  exact mdp_closed h₁ h₂;
+
+end Logic
+
+end LO.Propositional
